{
 "cells": [
  {
   "cell_type": "markdown",
   "id": "1848c388-da8c-44c8-99d2-2c578a14f65f",
   "metadata": {},
   "source": [
    "# Chapter 0"
   ]
  },
  {
   "cell_type": "markdown",
   "id": "1e516287-f9cf-4826-a095-891717d4d1ce",
   "metadata": {},
   "source": [
    "## Exercise 5\n",
    "\n",
    "Show that if $a$ and $b$ are positive integers, then $ab = \\text{lcm}(a, b) \\cdot \\text{gcd}(a, b)$.\n",
    "\n",
    "### Lemma 1\n",
    "\n",
    "Let $a = p_1^{\\alpha_1} \\cdots p_k^{\\beta_k}$ and $b = p_1^{\\beta_1} \\cdots p_k^{\\beta_k}$ be positive integers, where each $\\alpha_i$ and $\\beta_i$ is a non-negative integer. Then\n",
    "\n",
    "$$\n",
    "\\begin{align}\n",
    "\\text{gcd}(a, b) &= p_1^{\\text{min}(\\alpha_1, \\beta_1)} \\cdots p_k^{\\text{min}(\\alpha_k, \\beta_k)} \\\\\n",
    "\\text{lcm}(a, b) &= p_1^{\\text{max}(\\alpha_1, \\beta_1)} \\cdots p_k^{\\text{max}(\\alpha_k, \\beta_k)}.\n",
    "\\end{align}\n",
    "$$\n",
    "\n",
    "*Proof.*  Let $d=p_1^{\\text{min}(\\alpha_1, \\beta_1)} \\cdots p_k^{\\text{min}(\\alpha_k, \\beta_k)}$. Further, let $\\mu_i = \\text{min}(\\alpha_i, \\beta_i)$ for each $i$. To show $d | a$, note that $\\mu_i \\le \\alpha_i$, so there is some non-negative integer $\\gamma_i$ such that $\\mu_i + \\gamma_i = \\alpha_i$. Setting $c := p_1^{\\gamma_1} \\cdots p_k^{\\gamma_k}$, this means\n",
    "\n",
    "$$\n",
    "\\begin{align}\n",
    "a &= p_1^{\\mu_1 + \\gamma_1} \\cdots p_k^{\\mu_k + \\gamma_k} \\\\\n",
    "&= (p_1^{\\mu_1} \\cdots p_k^{\\mu_k})(p_k^{\\gamma_1} \\cdots p_k^{\\gamma_k}) \\\\\n",
    "&= dc.\n",
    "\\end{align}\n",
    "$$\n",
    "\n",
    "So, $d$ divides $a$. A similar argument follows to show $d$ divides $b$. Thus, $d$ is a common divisor of $a$ and $b$.\n",
    "\n",
    "To show $d$ is the greatest common divisor, suppose $d'$ is a common divisor of $a$ and $b$ (if $d'<0$, choose $-d'> 0$ instead). This means there are integers $e$ and $f$ such that $d'e=a$ and $d'f=b$. By unique factorization, we know $d' = p_1^{\\delta_1} \\cdots p_k^{\\delta_k}$, with each $\\delta_i \\ge 0$. Similarly, $e = p_1^{\\epsilon_1} \\cdots p_k^{\\epsilon_k}$ and $f = p_1^{\\phi_1} \\cdots p_k^{\\phi_k}$ with each $\\epsilon_i \\ge 0$ and $\\phi_i \\ge 0$. Then,\n",
    "\n",
    "$$\n",
    "\\begin{align}\n",
    "d'e &= (p_1^{\\delta_1} \\cdots p_k^{\\delta_k})(p_1^{\\epsilon_1} \\cdots p_k^{\\epsilon_k}) \\\\\n",
    "&= p_1^{\\delta_1 + \\epsilon_1} \\cdots p_k^{\\delta_k + \\epsilon_k} \\\\\n",
    "&= p_1^{\\alpha_1} \\cdots p_k^{\\alpha_k} \\\\\n",
    "&= a\n",
    "\\end{align}\n",
    "$$\n",
    "\n",
    "and\n",
    "\n",
    "$$\n",
    "\\begin{align}\n",
    "d'f &= (p_1^{\\delta_1} \\cdots p_k^{\\delta_k})(p_1^{\\phi_1} \\cdots p_k^{\\phi_k}) \\\\\n",
    "&= p_1^{\\delta_1 + \\phi_1} \\cdots p_k^{\\delta_k + \\phi_k} \\\\\n",
    "&= p_1^{\\beta_1} \\cdots p_k^{\\beta_k} \\\\\n",
    "&= b.\n",
    "\\end{align}\n",
    "$$\n",
    "\n",
    "In turn, by unique factorization again, $\\delta_i + \\epsilon_i = \\alpha_i$ and $\\delta_i + \\phi_i = \\beta_i$, so $\\delta_i \\le \\alpha_i$ and $\\delta_i \\le \\beta_i$ for each $i$. It follows that $\\delta_i \\le \\mu_i$ for each $i$. Again, this implies there is some non-negative integer $\\zeta_i$ such that $\\delta_i + \\zeta_i = \\mu_i$ for each $i$. As we have already seen, this means we have some integer $z$ such that $d'z=d$, so $d'|d$. Therefore, out of all the common divisors of $a$ and $b$, we have $d$ as the greatest.\n",
    "\n",
    "An analogous argument can also show $\\text{lcm}(a, b) = p_1^{\\text{max}(\\alpha_1, \\beta_1)} \\cdots p_k^{\\text{max}(\\alpha_k, \\beta_k)}$.\n",
    "\n",
    "### Lemma 2\n",
    "\n",
    "Let $x$ and $y$ be integers. Then $\\text{min}(x, y) + \\text{max}(x, y) = x + y$.\n",
    "\n",
    "*Proof.* Suppose $x \\le y$. Then $\\text{min}(x, y) = x$ and $\\text{max}(x, y) = y$. We then have $\\text{min}(x, y) + \\text{max}(x, y) = x + y$. In the alternate case $x \\gt y$, then $\\text{min}(x, y) = y$ and $\\text{max}(x, y) = x$. We again deduce $\\text{min}(x, y) + \\text{max}(x, y) = y + x = x + y$.\n",
    "\n",
    "### Solution\n",
    "\n",
    "Let $a = p_1^{\\alpha_1} \\cdots p_k^{\\beta_k}$ and $b = p_1^{\\beta_1} \\cdots p_k^{\\beta_k}$. With the help of our lemmas, we then have\n",
    "\n",
    "$$\n",
    "\\begin{align}\n",
    "ab &= (p_1^{\\alpha_1} \\cdots p_k^{\\beta_k})(p_1^{\\beta_1} \\cdots p_k^{\\beta_k}) \\\\\n",
    "   &= p_1^{\\alpha_1 + \\beta_1} \\cdots p_k^{\\alpha_k + \\beta_k} \\\\\n",
    "   &= p_1^{\\text{min}(\\alpha_1, \\beta_1) + \\text{max}(\\alpha_1, \\beta_1)} \\cdots p_k^{\\text{min}(\\alpha_k, \\beta_k) + \\text{max}(\\alpha_k, \\beta_k)} \\\\\n",
    "   &= (p_1^{\\text{max}(\\alpha_1, \\beta_1)} \\cdots p_k^{\\text{max}(\\alpha_k, \\beta_k)})(p_1^{\\text{min}(\\alpha_1, \\beta_1)} \\cdots p_k^{\\text{min}(\\alpha_k, \\beta_k)}) \\\\\n",
    "   &= \\text{lcm}(a, b) \\cdot \\text{gcd}(a, b).\n",
    "\\end{align}\n",
    "$$"
   ]
  },
  {
   "cell_type": "markdown",
   "id": "3f8132f3-1c77-4adf-8a3e-6d2caa94879d",
   "metadata": {},
   "source": [
    "## Exercise 6\n",
    "\n",
    "Suppose $a$ and $b$ are positive integers that divide the integer $c$. If $a$ and $b$ are relatively prime, show that $ab$ divides $c$. Show, by example, that if $a$ and $b$ are not relatively prime, then $ab$ need not divide $c$.\n",
    "\n",
    "### Solution\n",
    "\n",
    "Given $a \\mid c$, we have $ad = c$ for some integer $d$. Similarly, $bf = c$ for some $f$. At the same time, given $a$ and $b$ are coprime, there exists some integers $x$ and $y$ such that $ax + by = 1$. Multiplying both sides by $c$, we have $cax + cby = c$. Moreover, $cax + cby = bfax + adby = ab(fx + dy) = c$. As such, $ab \\mid c$.\n",
    "\n",
    "To show $ab$ neen not divide $c$ if $a$ and $b$ are not coprime, take $a = 4$, $b = 6$, and $c = 12$ for example. Of course, $4 \\mid 12$ and $6 \\mid 12$, but $4 \\cdot 6 = 24 \\nmid 12$. That is, in this case, $ab \\nmid c$."
   ]
  },
  {
   "cell_type": "markdown",
   "id": "a249680a-4634-4e4e-a8a1-2d35e04639a3",
   "metadata": {},
   "source": [
    "## Exercise 7\n",
    "\n",
    "If $a$ and $b$ are positive integers and $n$ is a positive integer, prove that $a \\mod n = b \\mod n$ if and only if $n$ divides $a - b$.\n",
    "\n",
    "### Solution\n",
    "\n",
    "Write $a = q_1n + r_1$ and $b = q_2n + r_2$ with $0 \\le r_1, r_2 \\lt n$ (the Division Algorithm allows us to do this). Suppose $a \\mod n = b \\mod n$. Given $a \\mod n = r_1$ and $b \\mod n = r_2$, we have $r_1 = r_2$. Further,\n",
    "\n",
    "$$a - b = q_1n + r_1 - (q_2n + r_2) = (q_1 - q_2)n + (r_1 - r_2) = (q_1 - q_2)n.$$\n",
    "\n",
    "So, $n$ divides $a - b$.\n",
    "\n",
    "For the converse, suppose $n$ divides $a - b$. Then there exists an integer $q$ such that $qn = a - b$. Consequently,\n",
    "\n",
    "$$\n",
    "\\begin{align}\n",
    "a &= qn + b \\\\\n",
    "  &= qn + q_2n + r_2 \\\\\n",
    "  &= (q + q_2)n + r_2\n",
    "\\end{align}\n",
    "$$\n",
    "\n",
    "with $0 \\le r_2 \\lt n$. Recall that $a = q_1n + r_1$ and $0 \\le r_1 \\lt n$. Given $q_1$ and $r_1$ are unique, we have $r_1 = r_2$, or $a \\mod n = b \\mod n$ as desired."
   ]
  },
  {
   "cell_type": "markdown",
   "id": "187d574c-385c-42cd-9917-0776985b770c",
   "metadata": {},
   "source": [
    "## Exercise 8\n",
    "\n",
    "Let $d = \\gcd(a, b)$. If $a = da'$ and $b = db'$, show that $\\gcd(a', b') = 1$.\n",
    "\n",
    "### Solution\n",
    "\n",
    "Given $d = \\gcd(a, b)$, then there exists integers $x$ and $y$ such that $ax + by = d$. That is, $da'x + db'y = d$. By cancellation, $a'x + b'y = 1$. (We know $d \\ne 0$ seeing that it is a divisor.) Of course, $1$ is the smallest positive integer that takes the form $a'x + b'y$, so $\\gcd(a', b') = 1$."
   ]
  },
  {
   "cell_type": "markdown",
   "id": "9026977a-166b-483f-9d88-53ed1af5496c",
   "metadata": {},
   "source": [
    "## Exercise 9\n",
    "\n",
    "Let $n$ be a fixed positive integer greater than $1$. If $a \\mod n = a'$ and $b \\mod n = b'$, prove that $(a + b) \\mod n = (a' + b') \\mod n$ and $(ab) \\mod n = (a'b') \\mod n$.\n",
    "\n",
    "### Solution\n",
    "\n",
    "We may write $a = q_1n + a'$ and $b = q_2n + b'$. Note that\n",
    "\n",
    "$$\n",
    "\\begin{align}\n",
    "(a + b) - (a' + b') &= a + b - a' - b' \\\\\n",
    "                    &= q_1n + a' + q_2n + b' - a' - b' \\\\\n",
    "                    &= (q_1 + q_2)n.\n",
    "\\end{align}\n",
    "$$\n",
    "\n",
    "Given $n \\mid (a + b) - (a' + b')$, then $(a + b) \\mod n = (a' + b') \\mod n$.\n",
    "\n",
    "Simultaneously, we have\n",
    "\n",
    "$$\n",
    "\\begin{align}\n",
    "ab - a'b' &= ab - a'b' \\\\\n",
    "          &= q_1q_2n^2 + b'q_1n + a'q_2n + a'b' - a'b' \\\\\n",
    "          &= (q_1q_2n + b'q_1 + a'q_2)n.\n",
    "\\end{align}\n",
    "$$\n",
    "\n",
    "Thus $n \\mid ab - a'b'$, so $(ab) \\mod n = (a'b') \\mod n$."
   ]
  },
  {
   "cell_type": "markdown",
   "id": "c2a98325-eba1-434e-90d6-d06fbad7ccc1",
   "metadata": {},
   "source": [
    "## Exercise 10\n",
    "\n",
    "Let $a$ and $b$ be positive integers and let $d = \\gcd (a, b)$ and $m = \\text{lcm} (a, b)$. If $t$ divides both $a$ and $b$, prove that $t$ divides $d$. If $s$ is a multiple of both $a$ and $b$, prove that $s$ is a multiple of $m$.\n",
    "\n",
    "### Solution\n",
    "\n",
    "Given $d = \\gcd (a, b)$, then $ax + by = d$ for some integers $x$ and $y$. At the same time, we have $t \\mid a$ and $t \\mid b$, so $tu = a$ and $tv = b$ for some integers $u$ and $v$. Thus, $ax + by = (tu)x + (tv)y = t(ux + vy) = d$, and $t$ divides $d$.\n",
    "\n",
    "We also have $m = \\text{lcm}(a, b)$ and $s$ as a multiple of both $a$ and $b$. We may write $s = qm + r$, where $0 \\le r \\lt m$. Again, $m$ and $s$ are multiples of $a$, so $s = aw$ and $m = az$ for some integers $w$ and $z$. Moreover, $aw = az + r$ and $aw - az = a(w - z) = r$. That is, $r$ is a multiple of $a$. A similar agrument shows that $r$ is also a multiple of $b$ and ultimately a common multiple of $a$ and $b$. Further, $0 \\lt r \\lt m$ contradicts that $m$ is the least common multiple of $a$ and $b$; we must have $r = 0$. Thus, $s = qm$ and $s$ is a multiple of $m$."
   ]
  },
  {
   "cell_type": "markdown",
   "id": "51133cee-972e-4628-8b74-34e14e115849",
   "metadata": {},
   "source": [
    "## Exercise 11\n",
    "\n",
    "Let $n$ and $a$ be positive integers and let $d = gcd(a, n)$. Show that the equation $ax \\mod n = 1$ has a solution if and only if $d = 1$.\n",
    "\n",
    "### Lemma\n",
    "\n",
    "If there exists integers $s$ and $t$ such that $as + bt = 1$, then $a$ and $b$ are relatively prime. (Converse of Theorem 0.2, Corollary 1.)\n",
    "\n",
    "*Proof.* Suppose there exists integers $s$ and $t$ such that $as + bt = 1$. Also suppose $d' = \\gcd (a, b)$. Then $d'u = a$ and $d'v = b$ for integers $u$ and $v$. Then $as + bt = d'us + d'vt = d'(us + vt) = 1$ and $d' \\mid 1$, so $d' = 1$.\n",
    "\n",
    "### Solution\n",
    "\n",
    "Suppose $ax \\mod n = 1$ for some integer $x$. Then $ax = qn + 1$ for some integer $q$. Further, $ax - qn = ax + (-q)n = 1$. By our Lemma, $d = gcd(a, n) = 1$.\n",
    "\n",
    "Suppose $d = 1$, then there are integers $x'$ and $q'$ such that $ax' + q'n = 1$. That is, $ax' = (-q')n + 1$. Simply choose $x := x'$ so we have $ax = (-q')n + 1$ and $ax \\mod n = 1$."
   ]
  },
  {
   "cell_type": "markdown",
   "id": "bfb8c6c7-069c-41bf-88d0-e4691a8fd917",
   "metadata": {},
   "source": [
    "## Exercise 12\n",
    "\n",
    "Show that $5n + 3$ and $7n + 4$ are relatively prime for all $n$.\n",
    "\n",
    "### Solution\n",
    "\n",
    "To prove $5n + 3$ and $7n + 4$ are relatively prime for all $n$, it suffices to show there exists integers $x$ and $y$ such that $(5n + 3)x + (7n + 4)y = 1$ (see Lemma of previous exercise). Choose $x := 7$ and $y := -5$. Then \n",
    "\n",
    "$$\n",
    "(5n + 3) \\cdot 7 + (7n + 4) \\cdot (-5) = 35n + 21 - 35n - 20 = 1.\n",
    "$$\n",
    "\n",
    "Thus, $5n + 3$ and $7n + 4$ are relatively prime.\n",
    "\n",
    "### Note\n",
    "\n",
    "It is assumed $n$ is any integer. Recall that Gallian's definition of relative primes does not require either number to be positive, only nonzero. So this proof may extend to the case where $n < 0$."
   ]
  },
  {
   "cell_type": "markdown",
   "id": "c2834bc7-a1ef-452e-8ec6-d02043ff1860",
   "metadata": {},
   "source": [
    "## Exercise 13\n",
    "\n",
    "Suppose that $m$ and $n$ are relatively prime and $r$ is any integer. Show that there are integers $x$ and $y$ such that $mx + ny = r$.\n",
    "\n",
    "### Solution\n",
    "\n",
    "Given $m$ and $n$ are relatively prime, then there are integers $a$ and $b$ where $ma + nb = 1$. Multiplying both sides by $r$, we have $m(ar) + n(br) = r$. Thus, there are integers $x = ar$ and $y = br$ such that $mx + ny = r$."
   ]
  },
  {
   "cell_type": "markdown",
   "id": "280c2670-613a-4418-a95c-7f0860ef16c1",
   "metadata": {},
   "source": [
    "## Exercise 14\n",
    "\n",
    "Let $p$, $q$, and $r$ be primes other than $3$. Show that $3$ divides $p^2 + q^2 + r^2$.\n",
    "\n",
    "### Lemma\n",
    "\n",
    "If $p$ is a prime other than $3$, then $p^2 \\mod 3 = 1$.\n",
    "\n",
    "We may write $p = 3a + r$ with $0 \\le r \\lt 3$. Given $p$ is prime, we have $p = 3a + 1$ or $p = 3a + 2$. (Note, $p = 3a + 0$ implies $3$ divides $p$, which contradicts $p$ is a prime other that $p$.)\n",
    "\n",
    "In the case $p = 3a + 1$, then $p^2 = 9a^2 + 6a + 1 = 3(3a^2 + 2a) + 1$ and $p^2 \\mod 3 = 1$.\n",
    "\n",
    "In the case $p = 3a + 2$, then $p^2 = 9a^2 + 12a + 4 = 3(3a^2 + 4a + 1) + 1$ and $p^2 \\mod 3 = 1$\n",
    "\n",
    "### Solution\n",
    "\n",
    "By our Lemma, we may write $p^2 = 3a + 1$, $q^2 = 3b + 1$, and $r^2 = 3c + 1$. Then $p^2 + q^2 + r^2 = 3(a + b + c + 1)$, and $3$ divides $p^2 + q^2 + r^2$."
   ]
  },
  {
   "cell_type": "code",
   "execution_count": null,
   "id": "1633c938-5ba0-4c16-94ba-c5ce0f87ce61",
   "metadata": {},
   "outputs": [],
   "source": []
  }
 ],
 "metadata": {
  "kernelspec": {
   "display_name": "Python 3 (ipykernel)",
   "language": "python",
   "name": "python3"
  },
  "language_info": {
   "codemirror_mode": {
    "name": "ipython",
    "version": 3
   },
   "file_extension": ".py",
   "mimetype": "text/x-python",
   "name": "python",
   "nbconvert_exporter": "python",
   "pygments_lexer": "ipython3",
   "version": "3.11.4"
  }
 },
 "nbformat": 4,
 "nbformat_minor": 5
}
